theories/crypto/SplitRO2.ec
@@ -6,7 +6,7 @@ abstract theory Split.
 
   op dout : in_t -> out_t distr.
 
-  clone import FullRO as IdealAll with 
+  clone import FullRO as IdealAll with
     type in_t    <- in_t,
     type out_t   <- out_t,
     type d_in_t  <- d_in_t,
@@ -15,7 +15,7 @@ abstract theory Split.
 
 abstract theory SplitDomT.
 
-module type ROt = { 
+module type ROt = {
   include RO [-init]
   proc init (_ : in_t -> bool) : unit
 }.
@@ -28,7 +28,7 @@ module RO : ROt = {
     m <- empty;
   }
 
-  proc get(x : in_t) = {
+  proc get (x : in_t) = {
     var r;
 
     r <$ dout x;
@@ -38,19 +38,19 @@ module RO : ROt = {
     return (oget m.[x]);
   }
 
-  proc set(x : in_t, y : out_t) = {
+  proc set (x : in_t, y : out_t) = {
     m.[x] <- y;
   }
 
-  proc rem(x : in_t) = {
+  proc rem (x : in_t) = {
     m <- rem m x;
   }
 
-  proc sample(x : in_t) = {
+  proc sample (x : in_t) = {
     get(x);
   }
 
-  proc restrK() = {
+  proc restrK () = {
     return m;
   }
 }.
@@ -60,12 +60,13 @@ clone include MkROt.
 
 module type RO_DistinguisherT (G : ROt) = {
   proc get_test () : in_t -> bool {}
-  proc distinguish(_ : d_in_t): d_out_t
+  proc distinguish (_ : d_in_t): d_out_t
 }.
 
 module MainDT (D : RO_DistinguisherT) (RO : ROt) = {
-  proc distinguish(x) = {
+  proc distinguish (x) = {
     var t, r;
+
     t <@ D(RO).get_test();
     RO.init(t);
     r <@ D(RO).distinguish(x);
@@ -78,25 +79,25 @@ module RO_DOMt (ROT : RO) (ROF: RO) : ROt = {
   var test : in_t -> bool
 
   proc init (test': in_t -> bool) = { test <- test'; ROT.init(); ROF.init(); }
- 
-  proc get(x : in_t) = {
+
+  proc get (x : in_t) = {
     var r;
     if (test x) r <@ ROT.get(x);
     else r <@ ROF.get(x);
     return r;
   }
 
-  proc set(x : in_t, y : out_t) = {
+  proc set (x : in_t, y : out_t) = {
     if (test x) ROT.set(x, y);
     else ROF.set(x, y);
   }
 
-  proc rem(x : in_t) = {
+  proc rem (x : in_t) = {
     if (test x) ROT.rem(x);
     else ROF.rem(x);
   }
 
-  proc sample(x : in_t) = {
+  proc sample (x : in_t) = {
     if (test x) ROT.sample(x);
     else ROF.sample(x);
   }
@@ -107,29 +108,33 @@ clone MkRO as ROF.
 
 section PROOFS.
 
-declare module D: RO_DistinguisherT { RO, RO_DOMt , ROT.RO, ROF.RO }.
+declare module D: RO_DistinguisherT {RO, RO_DOMt, ROT.RO, ROF.RO}.
 
-equiv RO_split: 
-    MainDT(D,RO).distinguish ~ MainDT(D,RO_DOMt(ROT.RO,ROF.RO)).distinguish : 
-      ={glob D, x} ==> ={res, glob D} /\ RO.m{1} = union_map ROT.RO.m{2} ROF.RO.m{2} /\
-                     (forall x, x \in ROT.RO.m{2} => RO_DOMt.test{2} x ) /\
-                     (forall x, x \in ROF.RO.m{2} => ! RO_DOMt.test{2} x).
+equiv RO_split :
+  MainDT(D, RO).distinguish ~ MainDT(D, RO_DOMt(ROT.RO, ROF.RO)).distinguish :
+  ={arg, glob D} ==>
+  ={res, glob D} /\ RO.m{1} = union_map ROT.RO.m{2} ROF.RO.m{2} /\
+  (forall x, x \in ROT.RO.m{2} => RO_DOMt.test{2} x ) /\
+  (forall x, x \in ROF.RO.m{2} => ! RO_DOMt.test{2} x).
 proof.
   proc.
   call (_ : RO.m{1} = union_map ROT.RO.m{2} ROF.RO.m{2} /\
             (forall x, x \in ROT.RO.m{2} => RO_DOMt.test{2} x ) /\
             (forall x, x \in ROF.RO.m{2} => ! RO_DOMt.test{2} x)).
   - proc; inline *.
-    by if {2}; auto=> />; smt(get_setE mem_union_map set_union_map_l set_union_map_r mem_set mergeE).
+    if {2}; auto=> />; 2: smt(get_setE mergeE set_union_map_r).
+    by smt(get_setE mem_union_map mergeE set_union_map_l).
   - proc; inline *.
-    by if {2}; auto=> />; smt(get_setE mem_union_map set_union_map_l set_union_map_r mem_set mergeE).
-  - proc; inline *; auto=> />; smt(rem_id mem_rem rem_merge).
+    if {2}; auto=> />; 2: smt(get_setE mergeE set_union_map_r).
+    by smt(get_setE mem_union_map mergeE set_union_map_l).
+  - by proc; inline *; auto=> />; smt(mem_rem rem_id rem_merge).
   - proc; inline *.
-    by if {2}; auto=> />; smt(get_setE mem_union_map set_union_map_l set_union_map_r mem_set mergeE).
-  - proc; inline *. auto => />. 
+    if {2}; auto=> />; 2: smt(get_setE mergeE set_union_map_r).
+    by smt(get_setE mem_union_map mergeE set_union_map_l).
+  - proc; inline *; auto => />.
     by rewrite {1}/union_map merge_empty //; smt(mem_empty).
   - inline *; auto; call(: true) => />; 1: by move=> /> /#.
-    skip => /> r. by rewrite {1}/union_map merge_empty //; smt(mem_empty).
+    by skip => /> r; rewrite {1}/union_map merge_empty //; smt(mem_empty).
 qed.
 
 end section PROOFS.
